lib/GraphBasics/Dipaths.v
@@ -1,0 +1,939 @@
+(* This program is free software; you can redistribute it and/or      *)
+(* modify it under the terms of the GNU Lesser General Public License *)
+(* as published by the Free Software Foundation; either version 2.1   *)
+(* of the License, or (at your option) any later version.             *)
+(*                                                                    *)
+(* This program is distributed in the hope that it will be useful,    *)
+(* but WITHOUT ANY WARRANTY; without even the implied warranty of     *)
+(* MERCHANTABILITY or FITNESS FOR A PARTICULAR PURPOSE.  See the      *)
+(* GNU General Public License for more details.                       *)
+(*                                                                    *)
+(* You should have received a copy of the GNU Lesser General Public   *)
+(* License along with this program; if not, write to the Free         *)
+(* Software Foundation, Inc., 51 Franklin St, Fifth Floor, Boston, MA *)
+(* 02110-1301 USA                                                     *)
+
+
+
+(* Different definitions of pathes in a directed graph.                 *)
+
+(* The following notions are defined :                                  *)
+(*      - D_walk : list of vertices joined one by one by arcs,          *)
+(*                constructors : DW_null, DW_step;                      *)
+(*      - D_trail : walk without repetition of arcs,                    *)
+(*              constructors : DT_null, DT_step;                        *)
+(*      - D_path : trail without repetition of inner vertices,          *)
+(*              constructors : DP_null, DP_step;                        *)
+(*      - D_closed_walk, D_closed_trail, D_cycle.                       *)
+
+Require Export Digraphs.
+
+Section DIRECTED_PATHES.
+
+Variable A:Type.
+Variable v : @V_set A.
+Variable a : @A_set A.
+
+Inductive D_walk : @Vertex A-> @Vertex A-> @V_list A-> @A_list A-> Prop :=
+  | DW_null : forall x : Vertex, v x -> D_walk x x V_nil A_nil
+  | DW_step :
+      forall (x y z : Vertex) (vl : V_list) (al : A_list),
+      D_walk y z vl al ->
+      v x -> a (A_ends x y) -> D_walk x z (y :: vl) (A_ends x y :: al).
+
+Definition D_closed_walk :=
+  forall (x : Vertex) (vl : V_list) (al : A_list), D_walk x x vl al.
+
+Inductive D_trail : @Vertex A-> @Vertex A-> @V_list A-> @A_list A-> Prop :=
+  | DT_null : forall x : Vertex, v x -> D_trail x x V_nil A_nil
+  | DT_step :
+      forall (x y z : Vertex) (vl : V_list) (al : A_list),
+      D_trail y z vl al ->
+      v x ->
+      a (A_ends x y) ->
+      ~ In (A_ends x y) al -> D_trail x z (y :: vl) (A_ends x y :: al).
+
+Definition D_closed_trail :=
+  forall (x : Vertex) (vl : V_list) (al : A_list), D_trail x x vl al.
+
+Inductive D_path : @Vertex A-> @Vertex A-> @V_list A-> @A_list A-> Prop :=
+  | DP_null : forall x : Vertex, v x -> D_path x x V_nil A_nil
+  | DP_step :
+      forall (x y z : Vertex) (vl : V_list) (al : A_list),
+      D_path y z vl al ->
+      v x ->
+      a (A_ends x y) ->
+      x <> y ->
+      ~ In y vl ->
+      (In x vl -> x = z) ->
+      ~ In (A_ends x y) al -> D_path x z (y :: vl) (A_ends x y :: al).
+
+Definition D_cycle :=
+  forall (x : Vertex) (vl : V_list) (al : A_list), D_path x x vl al.
+
+
+Lemma D_trail_isa_walk :
+ forall (x y : Vertex) (vl : V_list) (al : A_list) (t : D_trail x y vl al),
+ D_walk x y vl al.
+Proof.
+        intros x y vl al t; elim t; intros.
+        apply DW_null; trivial.
+
+        apply DW_step; trivial.
+Qed.
+
+Lemma D_path_isa_trail :
+ forall (x y : Vertex) (vl : V_list) (al : A_list) (p : D_path x y vl al),
+ D_trail x y vl al.
+Proof.
+        intros x y vl al p; elim p; intros.
+        apply DT_null; trivial.
+
+        apply DT_step; trivial.
+Qed.
+
+Lemma D_path_isa_walk :
+ forall (x y : Vertex) (vl : V_list) (al : A_list) (p : D_path x y vl al),
+ D_walk x y vl al.
+Proof.
+   intros. apply D_trail_isa_walk. apply D_path_isa_trail; auto.
+Qed.
+
+Lemma DW_iny_vl :
+ forall (x y : Vertex) (vl : V_list) (al : A_list),
+ D_walk x y vl al -> vl <> V_nil -> In y vl.
+Proof.
+        intros x y vl al d; elim d; intros.
+        absurd (V_nil = @V_nil A); auto.
+
+        inversion H.
+        simpl in |- *; auto.
+
+        rewrite H9; simpl in |- *; right.
+        apply H0; rewrite <- H9; discriminate.
+Qed.
+
+Lemma DW_endx_inv :
+ forall (x y : Vertex) (vl : V_list) (al : A_list), D_walk x y vl al -> v x.
+Proof.
+        intros x y vl el d; elim d; auto.
+Qed.
+
+Lemma DW_endy_inv :
+ forall (x y : Vertex) (vl : V_list) (al : A_list), D_walk x y vl al -> v y.
+Proof.
+        intros x y vl el d; elim d; auto.
+Qed.
+
+Lemma DW_invl_inv :
+ forall (x y : Vertex) (vl : V_list) (al : A_list),
+ D_walk x y vl al -> forall z : Vertex, In z vl -> v z.
+Proof.
+        intros x y vl al d; elim d; intros.
+        inversion H0.
+
+        inversion H3; subst; auto.
+        apply (DW_endx_inv _ _ _ _ H).
+Qed.
+
+Lemma DW_inel_ina :
+ forall (x y : Vertex) (vl : V_list) (al : A_list),
+ D_walk x y vl al ->
+ forall x' y' : Vertex, In (A_ends x' y') al -> a (A_ends x' y').
+Proof.
+        intros x y vl el d; elim d; intros.
+        inversion H0.
+
+        inversion H3; auto.
+        inversion H4; subst; auto.
+Qed.
+
+Lemma DW_inxyel_inxvl :
+ forall (x y : Vertex) (vl : V_list) (al : A_list),
+ D_walk x y vl al ->
+ forall x' y' : Vertex, In (A_ends x' y') al -> In x' (x :: vl).
+Proof.
+        intros x y vl al d; elim d; intros.
+        inversion H0.
+
+        inversion H3.
+          inversion H4.
+          simpl in |- *; auto.
+
+          simpl in |- *; right.
+          apply (H0 x' y'); auto.
+Qed.
+
+Lemma DW_inxyel_inyvl :
+ forall (x y : Vertex) (vl : V_list) (al : A_list),
+ D_walk x y vl al ->
+ forall x' y' : Vertex, In (A_ends x' y') al -> In y' (x :: vl).
+Proof.
+        intros x y vl el d; elim d; intros.
+        inversion H0.
+
+        inversion H3.
+          inversion H4.
+          simpl in |- *; auto.
+
+          simpl in |- *; right.
+          apply (H0 x' y'); auto.
+Qed.
+
+Lemma DW_backstep :
+ forall (x y z : Vertex) (vl : V_list) (al : A_list),
+ D_walk x z (y :: vl) al ->
+   exists al' : A_list, D_walk y z vl al' /\ (al = (A_ends x y) ::al').
+Proof.
+        intros; inversion H.
+        split with al0. split; auto.
+Qed.
+
+Lemma DW_neq_ends_inv :
+ forall (x y : Vertex) (vl : V_list) (al : A_list),
+ D_walk x y vl al -> x <> y -> vl <> V_nil /\ al <> A_nil.
+Proof.
+        intros; inversion H; subst; auto.
+          split; intro J; inversion J.
+Qed.
+
+Lemma DW_Vnil_inv :
+ forall (x y : Vertex) (al : A_list),
+ D_walk x y V_nil al -> x = y /\ al = A_nil.
+Proof.
+        intros; inversion H; subst; auto.
+Qed.
+
+Lemma DW_Anil_inv :
+ forall (x y : Vertex) (vl : V_list),
+ D_walk x y vl A_nil -> x = y /\ vl = V_nil.
+Proof.
+        intros; inversion H; subst; auto.
+Qed.
+
+Lemma DP_iny_vl :
+ forall (x y : Vertex) (vl : V_list) (al : A_list),
+ D_path x y vl al -> vl <> V_nil -> In y vl.
+Proof.
+        intros x y vl al d; elim d; intros.
+        absurd (V_nil = @V_nil A); auto.
+
+        inversion H.
+          simpl in |- *; auto.
+
+          rewrite H17; simpl in |- *; right.
+          apply H0; rewrite <- H17; discriminate.
+Qed.
+
+Lemma DP_endx_inv :
+ forall (x y : Vertex) (vl : V_list) (al : A_list), D_path x y vl al -> v x.
+Proof.
+        intros x y vl el d; elim d; auto.
+Qed.
+
+Lemma DP_endy_inv :
+ forall (x y : Vertex) (vl : V_list) (al : A_list), D_path x y vl al -> v y.
+Proof.
+        intros x y vl el d; elim d; auto.
+Qed.
+
+Lemma DP_invl_inv :
+ forall (x y : Vertex) (vl : V_list) (al : A_list),
+ D_path x y vl al -> forall z : Vertex, In z vl -> v z.
+Proof.
+        intros x y vl al d; elim d; intros.
+        inversion H0.
+
+        inversion H7; subst; auto.
+        apply (DP_endx_inv _ _ _ _ H).
+Qed.
+
+Lemma DP_inel_ina :
+ forall (x y : Vertex) (vl : V_list) (al : A_list),
+ D_path x y vl al ->
+ forall x' y' : Vertex, In (A_ends x' y') al -> a (A_ends x' y').
+Proof.
+        intros x y vl el d; elim d; intros.
+        inversion H0.
+
+        inversion H7; subst; auto.
+        inversion H8; subst; auto.
+Qed.
+
+Lemma DP_inxyel_inxvl :
+ forall (x y : Vertex) (vl : V_list) (al : A_list),
+ D_path x y vl al ->
+ forall x' y' : Vertex, In (A_ends x' y') al -> In x' (x :: vl).
+Proof.
+        intros x y vl al d; elim d; intros.
+        inversion H0.
+
+        inversion H7.
+          inversion H8; subst.
+          simpl in |- *; auto.
+
+          simpl in |- *; right.
+          apply (H0 x' y'); auto.
+Qed.
+
+Lemma DP_inxyel_inyvl :
+ forall (x y : Vertex) (vl : V_list) (al : A_list),
+ D_path x y vl al ->
+ forall x' y' : Vertex, In (A_ends x' y') al -> In y' (x :: vl).
+Proof.
+        intros x y vl el d; elim d; intros.
+        inversion H0.
+
+        inversion H7.
+          inversion H8; subst.
+          simpl in |- *; auto.
+
+          simpl in |- *; right.
+          apply (H0 x' y'); auto.
+Qed.
+
+Lemma DP_endx_ninV :
+ forall (x y : Vertex) (vl : V_list) (al : A_list),
+ D_path x y vl al -> x <> y -> ~ In x vl.
+Proof.
+  intros x y vl el d Hneq. inversion d; subst; simpl; auto.
+  intro J.
+  destruct J as [J | J]; subst; auto.
+Qed.
+
+Lemma DP_backstep :
+ forall (x y z : Vertex) (vl : V_list) (al : A_list),
+ D_path x z (y :: vl) al -> exists al' : A_list, D_path y z vl al'.
+Proof.
+        intros; inversion H.
+        split with al0; trivial.
+Qed.
+
+Lemma DP_prefix_no_head:  forall (y z : Vertex) (vl : V_list) (al : A_list) 
+ (H: D_path y z vl al), 
+ vl = V_nil \/ (exists vl', vl = vl' ++ z::nil /\ ~ In z vl').
+Proof.
+  intros.
+  induction H; auto.
+    right.
+    destruct IHD_path as [J | [vl' [J1 J2]]]; subst.
+      inversion H; subst.
+      exists nil. split; auto.
+
+      exists (y::vl').
+      split; auto.
+        simpl.
+        intro J.
+        destruct J as [J | J]; subst; auto.
+          apply H3. apply in_or_app; simpl; auto.
+Qed.
+
+End DIRECTED_PATHES.
+
+Implicit Arguments D_walk [A].
+Implicit Arguments DW_backstep [A].
+Implicit Arguments D_path [A].
+Implicit Arguments DP_backstep [A].
+Implicit Arguments DP_endx_inv [A].
+Implicit Arguments DP_inxyel_inxvl [A].
+
+Require Export Paths.
+
+Section DEXTRACTED.
+
+Variable A:Type.
+Variable eq_a_dec: forall x y : A, {x = y} + {x <> y}.
+
+Variable v : @V_set A.
+Variable a : @A_set A.
+
+Lemma DW_extract :
+ forall (x y z : Vertex) (vl : V_list) (al : A_list),
+ D_walk v a y z vl al ->
+ In x (y :: vl) ->
+ exists al' : A_list, D_walk v a x z (V_extract eq_a_dec x (y :: vl)) al'.
+Proof.
+        intros x y z vl; generalize y; elim vl; simpl in |- *; intros.
+        split with al.
+        replace x with y0; auto.
+        case (V_in_dec eq_a_dec y0 nil); auto.
+
+        tauto.
+
+        elim (DW_backstep _ _ _ _ _ _ _ H0); intros.
+        destruct H2 as [H2 Heq]; subst.
+        case (V_in_dec eq_a_dec x (a0 :: l)). intros.
+        apply (H a0 x0); auto.
+
+        simpl in |- *. intros.
+        split with (A_ends y0 a0 :: x0).
+        replace x with y0.
+          trivial.
+
+          tauto.
+Qed.
+
+Lemma DW_cut :
+ forall (y z: Vertex) (vl : V_list) (al : A_list),
+ D_walk v a y z vl al -> vl <> V_nil ->
+ forall x w,
+ In x (y :: vl) ->
+ In w (y :: vl) ->
+ x <> y -> w <> y -> x <> w ->
+    exists al1 : A_list, exists al2 : A_list, exists vl1 : V_list,
+    exists vl2 : V_list,
+      (D_walk v a y x vl1 al1 /\ D_walk v a x z vl2 al2 /\
+       (al1 ++ al2 = al) /\ (vl1 ++ vl2 = vl) /\ ~ In w (y::vl1)) \/
+      (D_walk v a y w vl1 al1 /\ D_walk v a w z vl2 al2 /\
+       (al1 ++ al2 = al) /\ (vl1 ++ vl2 = vl) /\ ~ In x (y::vl1)).
+Proof.
+  induction 1; simpl in *; intros.
+    congruence.
+
+    destruct H3 as [H3 | H3]; try congruence; subst.
+    destruct H4 as [H4 | H4]; try congruence; subst.
+    destruct vl.
+      inversion H; subst.
+      destruct H3 as [H3 | H3]; try solve [inversion H3]; subst.
+      destruct H4 as [H4 | H4]; try solve [inversion H4]; subst.
+      congruence.
+
+      destruct (V_eq_dec eq_a_dec y w); subst.
+        exists (A_ends x w::nil). exists al. exists (w::nil). exists (v0::vl).
+        right.
+        split. constructor; auto. constructor; auto. apply DW_endx_inv in H; auto.
+        split; auto.
+        split; auto.
+        split; auto.
+          intro J.
+          destruct J as [J | J]; subst.
+            congruence.
+            simpl in J.
+            destruct J as [J | J]; subst; auto.
+
+      destruct (V_eq_dec eq_a_dec y x0); subst.
+        exists (A_ends x x0::nil). exists al. exists (x0::nil). exists (v0::vl).
+        left.
+        split. constructor; auto. constructor; auto. apply DW_endx_inv in H; auto.
+        split; auto.
+        split; auto.
+        split; auto.
+          intro J.
+          destruct J as [J | J]; subst.
+            congruence.
+            simpl in J.
+            destruct J as [J | J]; subst; auto.
+
+          eapply IHD_walk in H3; eauto.
+            clear IHD_walk.
+            destruct H3 as [al1 [al2 [vl1 [vl2
+              [[J1 [J2 [J3 [J4 J5]]]]|[J1 [J2 [J3 [J4 J5]]]]]]]]]; subst.
+              exists (A_ends x y::al1). exists al2. exists (y::vl1). exists vl2.
+              right. rewrite <- J4.
+              split. constructor; auto.
+              split; auto.
+              split; auto.
+              split; auto.
+                intro J.
+                destruct J as [J | J]; subst.
+                  congruence.
+                  apply J5. simpl in J. auto.
+
+              exists (A_ends x y::al1). exists al2. exists (y::vl1). exists vl2.
+              left. rewrite <- J4.
+              split. constructor; auto.
+              split; auto.
+              split; auto.
+              split; auto.
+                intro J.
+                destruct J as [J | J]; subst.
+                  congruence.
+                  apply J5. simpl in J. auto.
+            intro J. inversion J.
+Qed.
+
+Lemma DW_split :
+ forall (x y z : Vertex) (vl : V_list) (al : A_list),
+ D_walk v a y z vl al ->
+ In x (y :: vl) ->
+    exists al1 : A_list, exists al2 : A_list, exists vl1 : V_list,
+    exists vl2 : V_list,
+      D_walk v a y x vl1 al1 /\ D_walk v a x z vl2 al2 /\
+      (al1 ++ al2 = al) /\ (vl1 ++ vl2 = vl).
+Proof.
+  intros.
+  induction H.
+    assert (x0 = x) as EQ.
+      simpl in H0.
+      destruct H0 as [H0 | H0]; inversion H0; auto.
+    clear H0. subst.
+    exists A_nil. exists A_nil. exists V_nil. exists V_nil.
+    repeat split; try solve [auto | constructor; auto].
+
+    destruct (V_eq_dec eq_a_dec x x0); subst.
+      exists A_nil. exists (A_ends x0 y :: al). exists V_nil. exists (y::vl).
+      repeat split; try solve [auto | constructor; auto].
+
+      assert (In x (y::vl)) as Hin.
+        simpl in H0.
+        destruct H0 as [H0 | H0]; auto; try congruence.
+      clear H0.
+      apply IHD_walk in Hin.
+      destruct Hin as [al1 [al2 [vl1 [vl2 [J1 [J2 [J3 J4]]]]]]]; subst.
+      exists (A_ends x0 y::al1). exists al2. exists (y::vl1). exists vl2.
+      repeat split; try solve [auto | constructor; auto].
+Qed.
+
+Lemma DP_extract :
+ forall (x y z : Vertex) (vl : V_list) (al : A_list),
+ D_path v a y z vl al ->
+ In x (y :: vl) ->
+ exists al' : A_list,  D_path v a x z (V_extract eq_a_dec x (y :: vl)) al'.
+Proof.
+        intros x y z vl; generalize y; elim vl; simpl in |- *; intros.
+        split with al.
+        replace x with y0; auto.
+        case (V_in_dec eq_a_dec y0 nil); auto.
+
+        tauto.
+
+        elim (DP_backstep _ _ _ _ _ _ _ H0); intros.
+        case (V_in_dec eq_a_dec x (a0 :: l)). intros.
+        apply (H a0 x0); auto.
+
+        simpl in |- *. intros. split with al. replace x with y0.
+        trivial.
+
+        tauto.
+Qed.
+
+Remark DP_when_cycle :
+ forall (x y : Vertex) (vl : V_list) (al : A_list),
+ D_path v a x y vl al -> In x vl -> x = y.
+Proof.
+        intros x y vl al H; inversion H; intros.
+        trivial.
+
+        inversion H11.
+        absurd (x = y0); auto.
+
+        auto.
+Qed.
+
+Lemma DP_split :
+ forall v a (x y z : Vertex) (vl : V_list) (al : A_list) 
+ (H: D_path v a y z vl al),
+ In x (y :: vl) ->
+    exists al1 : A_list, exists al2 : @A_list A, exists vl1 : V_list,
+    exists vl2 : V_list,
+      D_path v a y x vl1 al1 /\ D_path v a x z vl2 al2 /\
+      (al1 ++ al2 = al) /\ (vl1 ++ vl2 = vl).
+Proof.
+  intros.
+  induction H; intros.
+    assert (x0 = x) as EQ.
+      simpl in H0.
+      destruct H0 as [H0 | H0]; inversion H0; auto.
+    clear H0. subst.
+    exists A_nil. exists A_nil. exists V_nil. exists V_nil.
+    repeat split; try solve [auto | constructor; auto].
+
+    destruct (V_eq_dec eq_a_dec x x0); subst.
+      exists A_nil. exists (A_ends x0 y :: al). exists V_nil. exists (y::vl).
+      repeat split; try solve [auto | constructor; auto].
+
+      assert (In x (y::vl)) as Hin.
+        simpl in H0.
+        destruct H0 as [H0 | H0]; auto; try congruence.
+      clear H0.
+      apply IHD_path in Hin; auto.
+      destruct Hin as [al1 [al2 [vl1 [vl2 [J1 [J2 [J3 J4]]]]]]]; subst.
+      exists (A_ends x0 y::al1). exists al2. exists (y::vl1). exists vl2.
+      repeat split; try solve [auto | constructor; auto].
+      constructor; auto.
+        intro J. apply H4. apply in_or_app. auto.
+
+        intro J. 
+        assert (In x0 (vl1++vl2)) as Hin. 
+          apply in_or_app. auto.
+        apply H5 in Hin. subst. 
+        assert (J2':=J2).
+        apply DP_prefix_no_head in J2'.
+        destruct J2' as [EQ | [vl' [EQ Hnotin]]]; subst.
+          inversion J2; subst; auto.
+          
+          apply DP_prefix_no_head in H.
+          destruct H as [EQ | [v2' [EQ Hnotin']]]; subst.
+            assert (In z V_nil) as G.
+              rewrite <- EQ.
+              apply in_or_app. right. apply in_or_app; simpl; auto.
+            inversion G.
+        
+            rewrite app_assoc in EQ.
+            apply app_inj_tail in EQ.
+            destruct EQ; subst.
+            contradict Hnotin'.
+            apply in_or_app; auto.
+        
+        intro J. apply H6. apply in_or_app. auto.
+Qed.
+
+Lemma DWalk_to_dpath' :
+ forall (x y : Vertex) (vl : V_list) (al : A_list),
+ D_walk v a x y vl al ->
+ exists vl0 : V_list, exists al0 : A_list, 
+    D_path v a x y vl0 al0 /\
+    (forall vx, In vx vl0 -> In vx vl).
+Proof.
+  intros x y vl al w; elim w; intros.
+    split with V_nil; split with A_nil. 
+    split; auto.
+     apply DP_null; trivial.
+
+    elim H0; clear H0; intros vl' H0.
+    elim H0; clear H0; intros al' H0.
+    destruct H0 as [H0 Hinv].           
+    case (V_in_dec eq_a_dec x0 (y0 :: vl')); intros.
+      elim (DP_extract _ _ _ _ _ H0 i); intros.
+      split with (V_extract eq_a_dec x0 (y0 :: vl')); split with x1.
+      split; auto.
+        intros vx Hinvx.
+        apply V_extract_spec'' in Hinvx.
+        simpl in *.
+        destruct Hinvx; auto.
+
+      case (V_in_dec eq_a_dec y0 vl'); intros.
+        split with (y0 :: V_nil); split with (A_ends x0 y0 :: A_nil).
+        split; try solve [
+           intros vx Hinvx; simpl in Hinvx; simpl; destruct Hinvx; 
+           try solve [auto | tauto]
+        ].
+        apply DP_step.
+          replace z with y0.
+            apply DP_null; apply (DP_endx_inv _ _ _ _ _ _ H0).
+
+            apply (DP_when_cycle _ _ _ _ H0); auto.
+
+          trivial.
+
+          trivial.
+
+          red in |- *; intros; elim n; subst; simpl in |- *; auto.
+
+          tauto.
+
+          simpl in |- *. tauto.
+
+          tauto.
+
+        split with (y0 :: vl'); split with (A_ends x0 y0 :: al').
+        split; try solve [
+           intros vx Hinvx; simpl in Hinvx; simpl; destruct Hinvx; auto
+        ].
+        apply DP_step.
+          trivial.
+
+          trivial.
+
+          trivial.
+
+          red in |- *; intros; elim n; subst; simpl in |- *; auto.
+
+          trivial.
+
+          intros; absurd (In x0 vl').
+            red in |- *; intros; elim n; simpl in |- *; auto.
+
+            trivial.
+
+            red in |- *; intros.
+            elim n; inversion w; apply (DP_inxyel_inxvl _ _ _ _ _ _ H0 x0 y0); auto.
+Qed.
+
+Lemma DWalk_to_dpath :
+ forall (x y : Vertex) (vl : V_list) (al : A_list),
+ D_walk v a x y vl al ->
+ exists vl0 : V_list, exists al0 : A_list, D_path v a x y vl0 al0.
+Proof.
+  intros.
+  apply DWalk_to_dpath' in H.
+  destruct H as [? [? [? ?]]]; eauto.
+Qed.
+
+End DEXTRACTED.
+
+Implicit Arguments D_trail [A].
+
+Section DPATH_EQ.
+
+Variable A:Type.
+
+Lemma DWalk_eq :
+ forall (v v' : V_set) (a a' : @A_set A) (x y : Vertex)
+   (vl : V_list) (al : A_list),
+ D_walk v a x y vl al -> v = v' -> a = a' -> D_walk v' a' x y vl al.
+Proof.
+        intros; elim H; intros.
+        apply DW_null.
+        rewrite <- H0; trivial.
+
+        apply DW_step.
+        trivial.
+
+        rewrite <- H0; trivial.
+
+        rewrite <- H1; trivial.
+Qed.
+
+Lemma DTrail_eq :
+ forall (v v' : V_set) (a a' : @A_set A) (x y : Vertex)
+   (vl : V_list) (al : A_list),
+ D_trail v a x y vl al -> v = v' -> a = a' -> D_trail v' a' x y vl al.
+Proof.
+        intros; elim H; intros.
+        apply DT_null.
+        rewrite <- H0; trivial.
+
+        intros; apply DT_step.
+        trivial.
+
+        rewrite <- H0; trivial.
+
+        rewrite <- H1; trivial.
+
+        trivial.
+Qed.
+
+Lemma DPath_eq :
+ forall (v v' : V_set) (a a' : @A_set A) (x y : Vertex)
+   (vl : V_list) (al : A_list),
+ D_path v a x y vl al -> v = v' -> a = a' -> D_path v' a' x y vl al.
+Proof.
+        intros; elim H; intros.
+        apply DP_null.
+        rewrite <- H0; trivial.
+
+        intros; apply DP_step.
+        trivial.
+
+        rewrite <- H0; trivial.
+
+        rewrite <- H1; trivial.
+
+        trivial.
+
+        trivial.
+
+        trivial.
+
+        trivial.
+Qed.
+
+End DPATH_EQ.
+
+Section APPEND_DWALKS.
+
+Variable A:Type.
+Variable v : @V_set A.
+Variable a : @A_set A.
+
+Lemma DWalk_append :
+ forall (x y z : Vertex) (vl vl' : V_list) (al al' : A_list),
+ D_walk v a x y vl al ->
+ D_walk v a y z vl' al' -> D_walk v a x z (vl ++ vl') (al ++ al').
+Proof.
+        intros x y z vl vl' al al' Hw; elim Hw; simpl in |- *; intros.
+        trivial.
+
+        apply DW_step; auto.
+Qed.
+
+End APPEND_DWALKS.
+
+Lemma D_walk_iff: forall A v1 a1 x y vl al v2 a2
+  (H1: forall x, v2 x <-> v1 x)
+  (H2: forall x, a2 x <-> a1 x),
+  @D_walk A v1 a1 x y vl al <->
+  D_walk v2 a2 x y vl al.
+Proof.
+  intros.
+  split; intro J.
+    induction J; constructor; auto.
+      apply H1; auto.
+      apply H1; auto.
+      apply H2; auto.
+    induction J; constructor; auto.
+      apply H1; auto.
+      apply H1; auto.
+      apply H2; auto.
+Qed.
+
+Lemma D_walk_sub: forall A x y vl al (v1 v2:@V_set A) (a1 a2:@A_set A)
+  (H1: forall x, v2 x -> v1 x)
+  (H2: forall x, a2 x -> a1 x)
+  (J: @D_walk A v2 a2 x y vl al),
+  D_walk v1 a1 x y vl al.
+Proof.
+  intros.
+  induction J; constructor; auto.
+Qed.
+
+Require Import Metatheory.
+Require Import util.
+Require Import vellvm_tactics.
+
+Lemma DW_last_split: forall (A:Type) 
+  v a vl v1 v2 (al : @A_list A) 
+  (Hw : D_walk v a v2 v1 (vl ++ v1::nil) al),
+  exists v1', exists al',
+    D_walk v a v2 v1' vl al' /\
+    D_walk v a v1' v1 (v1::nil) (A_ends v1' v1::nil) /\
+    al = al' ++ (A_ends v1' v1::nil).
+Proof.
+  induction vl; intros.
+  (*base*)
+    assert (v v1) as J.
+      apply DW_endy_inv in Hw; auto.
+    inversion Hw; subst. inversion H1; subst.
+    exists v2. exists nil.
+    split.
+      constructor; auto.
+    split; auto.
+  (*ind*)
+    inversion Hw; subst.
+    apply IHvl in H1; auto.
+    destruct H1 as [v1' [al2 [Hw1 [Hw2 EQ]]]]; subst.
+    exists v1'. exists (A_ends v2 a0::al2).
+    split; auto.
+      constructor; auto. 
+Qed.
+
+Lemma DW_head_inversion :
+ forall A v a (z: Vertex) (vl : @V_list A) (x: Vertex) (al : @A_list A)
+ (Hw: D_walk v a x z vl al) (Hnnil: vl <> nil),
+ exists y, exists vl', exists al',
+   D_walk v a x y vl' al' /\
+   vl = vl' ++ (z::nil) /\
+   al = al' ++ (A_ends y z::nil) /\
+   a (A_ends y z) /\ v y.
+Proof.
+  intros.
+  apply nnil_inv in Hnnil.
+  destruct Hnnil as [vl' [v' EQ]]; subst.
+  generalize dependent x.
+  generalize dependent al.
+  induction vl'; intros.
+  (*base*)
+    assert (v z) as J.
+      apply DW_endy_inv in Hw; auto.
+    inversion Hw; subst. inversion H1; subst.
+    exists x. exists nil. exists nil.
+    split.
+      constructor; auto.
+    split; auto.
+  (*ind*)
+    inversion Hw; subst.
+    apply IHvl' in H1; auto.
+    destruct H1 as [v1' [vl2 [al2 [Hw1 [Hw2 [EQ1 [EQ2 J]]]]]]]; subst.
+    exists v1'. exists (a0::vl2). exists (A_ends x a0::al2).
+    split. constructor; auto. 
+    split. simpl_env. rewrite Hw2. auto. 
+    split; auto.
+Qed.
+
+Lemma DW_Forall_head: forall A v (a:@A_set A) v1 v2 vl al P 
+  (Hw: D_walk v a v1 v2 vl al)
+  (Hforall: Forall P (v1 :: vl)), P v2.
+Proof.
+  intros.
+  apply Forall_forall with (x:=v2) in Hforall; auto.
+  assert (Hw':=Hw).
+  inversion Hw; subst.
+    simpl; auto.
+
+    apply DW_iny_vl in Hw'.
+      simpl in *. tauto.
+
+      intro J. inversion J.
+Qed.
+
+Lemma DW_split' :
+ forall A v a (x z : Vertex) vl1 vl2 (vl : @V_list A) (al : @A_list A) 
+ (y: Vertex),
+ D_walk v a y z vl al ->
+ vl = vl2 ++ x :: vl1 ->
+    exists al1 : A_list, exists al2 : A_list, 
+      D_walk v a x z vl1 al1 /\ D_walk v a y x (vl2 ++ [x]) al2 /\
+      (al2 ++ al1 = al).
+Proof.
+  induction vl2; intros; subst.
+  Case "base".
+    inversion H; subst.
+    exists al0. exists [A_ends y x].
+    split; auto.
+    split; auto.
+      constructor; auto.
+      constructor; auto.
+        apply DW_endx_inv in H2; auto.
+  Case "ind".
+    simpl_env in H.
+    inversion H; subst.
+    apply IHvl2 in H2; auto.
+    destruct H2 as [al1 [al2 [Hw1 [Hw2 EQ]]]]; subst.
+    exists al1. exists (A_ends y a0::al2).
+    split; auto.
+    split; auto.
+      simpl_env. simpl. constructor; auto.     
+Qed.
+
+Lemma DW_split'' :
+ forall A v a (x z : Vertex) (vl : @V_list A) (al : @A_list A) 
+ (y: Vertex) (Hw: D_walk v a y z vl al) (Hin: In x vl),
+ exists vl2, exists vl1, exists al1 : A_list, exists al2 : A_list, 
+   vl = vl2 ++ x :: vl1 /\
+   D_walk v a x z vl1 al1 /\ D_walk v a y x (vl2 ++ [x]) al2 /\
+   (al2 ++ al1 = al).
+Proof.
+  intros.
+  apply in_split in Hin.
+  destruct Hin as [vl2 [vl1 EQ]].
+  exists vl2. exists vl1.
+  eapply DW_split' in Hw; eauto.
+  destruct Hw as [al1 [al2 [Hw1 [Hw2 EQ']]]].
+  exists al1. exists al2. auto.
+Qed.
+
+Lemma DW_chunk :
+ forall A v a (x z : Vertex) vl1 vl3 vl2 (vl : @V_list A) (al : @A_list A) 
+ (y: Vertex) (Hw: D_walk v a y z vl al) 
+ (EQ: y :: vl = vl2 ++ x :: vl3 ++ x :: vl1),
+ exists al3 : A_list, D_walk v a x x (vl3 ++ [x]) al3.
+Proof.
+  intros.
+  destruct vl2; inversion EQ; subst.
+  Case "base".
+    eapply DW_split' in Hw; eauto.
+    destruct Hw as [al1 [al2 [Hw1 [Hw2 EQ']]]]; subst. eauto.
+  Case "ind".
+    eapply DW_split' in Hw; eauto.
+    destruct Hw as [al1 [al2 [Hw1 [Hw2 EQ']]]]; subst. 
+    eapply DW_split' in Hw1; eauto.
+    destruct Hw1 as [al11 [al12 [Hw11 [Hw12 EQ']]]]; subst. eauto.
+Qed.
+
+Lemma D_walk_weakening: forall A x y vl al (v1 v2:@V_set A) (a1 a2:@A_set A)
+  (H1: forall z, In z (x::vl) -> v1 z)
+  (H2: forall z, In z al -> a1 z)
+  (J: @D_walk A v2 a2 x y vl al),
+  D_walk v1 a1 x y vl al.
+Proof.
+  intros.
+  induction J; constructor.
+    apply H1; simpl; auto.
+    apply IHJ.
+      intros. apply H1. simpl; auto.
+      intros. apply H2. simpl; auto.
+    apply H1; simpl; auto.
+    apply H2; simpl; auto.
+Qed.
+ 
