lib/compcert-2.4/common/Memory.v
@@ -38,9 +38,7 @@ Require Import Floats.
 Require Import Values.
 Require Export Memdata.
 Require Export Memtype.
-(* 1. eliminate signed
-2. nat -> ...
-*)
+
 (* To avoid useless definitions of inductors in extracted code. *)
 Local Unset Elimination Schemes.
 Local Unset Case Analysis Schemes.
@@ -269,6 +267,7 @@ Proof.
   intros. destruct H. apply perm_cur. apply H. generalize (size_chunk_pos chunk). omega.
 Qed.
 
+(* NOTE: not used
 Lemma valid_access_compat:
   forall m chunk1 chunk2 b ofs p,
   size_chunk chunk1 = size_chunk chunk2 ->
@@ -279,6 +278,7 @@ Proof.
   intros. inv H1. rewrite H in H2. constructor; auto.
   eapply Zdivide_trans; eauto. eapply align_le_divides; eauto.
 Qed.
+*)
 
 Lemma valid_access_dec:
   forall m chunk b ofs p,
@@ -308,13 +308,13 @@ Qed.
 
 Theorem valid_pointer_valid_access:
   forall m b ofs,
-  valid_pointer m b ofs = true <-> valid_access m Mint8 b ofs Nonempty.
+  valid_pointer m b ofs = true <-> valid_access m (Mint 7) b ofs Nonempty.
 Proof.
   intros. rewrite valid_pointer_nonempty_perm. 
   split; intros.
-  split. simpl; red; intros. replace ofs0 with ofs by omega. auto.
+  split. simpl; red; intros. unfold bytesize_chunk, ZRdiv, Zdiv in H0; simpl in H0. replace ofs0 with ofs by omega. auto.
   simpl. apply Zone_divide. 
-  destruct H. apply H. simpl. omega.
+  destruct H. apply H. simpl. unfold bytesize_chunk, ZRdiv, Zdiv; simpl; omega.
 Qed.
 
 (** C allows pointers one past the last element of an array.  These are not
@@ -455,7 +455,7 @@ Definition load (chunk: memory_chunk) (m: mem) (b: block) (ofs: Z): option val :
 
 Definition loadv (chunk: memory_chunk) (m: mem) (addr: val) : option val :=
   match addr with
-  | Vptr b ofs => load chunk m b (Int.unsigned ofs)
+  | Vptr b ofs => load chunk m b (Int.unsigned 31 ofs)
   | _ => None
   end.
 
@@ -571,7 +571,7 @@ Qed.
 
 Definition storev (chunk: memory_chunk) (m: mem) (addr v: val) : option mem :=
   match addr with
-  | Vptr b ofs => store chunk m b (Int.unsigned ofs) v
+  | Vptr b ofs => store chunk m b (Int.unsigned 31 ofs) v
   | _ => None
   end.
 
@@ -687,6 +687,7 @@ Proof.
   apply decode_val_type. 
 Qed.
 
+(* NOTE: not used
 Theorem load_cast:
   forall m chunk b ofs v,
   load chunk m b ofs = Some v ->
@@ -700,6 +701,7 @@ Proof.
   set (l := getN (size_chunk_nat chunk) ofs m.(mem_contents)#b).
   intros. subst v. apply decode_val_cast. 
 Qed.
+*)
 
 (** ** Properties related to [loadbytes] *)
 
@@ -846,6 +848,7 @@ Proof.
   rewrite inj_S. omega.
 Qed.
 
+(* NOTE: not used
 Theorem load_int64_split:
   forall m b ofs v,
   load Mint64 m b ofs = Some v ->
@@ -899,6 +902,7 @@ Opaque Int.repr.
   split. simpl. rewrite NV. auto. 
   auto.
 Qed.
+*)
 
 (** ** Properties related to [store] *)
 
@@ -999,6 +1003,7 @@ Qed.
 
 Local Hint Resolve store_valid_access_1 store_valid_access_2 store_valid_access_3: mem.
 
+(* NOTE: not used
 Theorem load_store_similar:
   forall chunk',
   size_chunk chunk' = size_chunk chunk ->
@@ -1035,6 +1040,7 @@ Theorem load_store_same:
 Proof.
   apply load_store_similar_2; auto. omega.
 Qed.
+*)
 
 Theorem load_store_other:
   forall chunk' b' ofs',
@@ -1179,20 +1185,22 @@ Qed.
 
 Definition compat_pointer_chunks (chunk1 chunk2: memory_chunk) : Prop :=
   match chunk1, chunk2 with
-  | (Mint32 | Many32), (Mint32 | Many32) => True
-  | Many64, Many64 => True
+  | Mint wz1, Mint wz2 =>
+    if eq_nat_dec 31 wz1 then
+      if eq_nat_dec 31 wz2 then True
+      else False
+    else False
   | _, _ => False
   end.
 
 Lemma compat_pointer_chunks_true:
   forall chunk1 chunk2,
-  (chunk1 = Mint32 \/ chunk1 = Many32 \/ chunk1 = Many64) ->
-  (chunk2 = Mint32 \/ chunk2 = Many32 \/ chunk2 = Many64) ->
+  chunk1 = Mint 31 ->
+  chunk2 = Mint 31 ->
   quantity_chunk chunk1 = quantity_chunk chunk2 ->
   compat_pointer_chunks chunk1 chunk2.
 Proof.
-  intros. destruct H as [P|[P|P]]; destruct H0 as [Q|[Q|Q]];
-  subst; red; auto; discriminate.
+  intros; subst; red; destruct (eq_nat_dec _ _); auto.
 Qed.
 
 Theorem load_pointer_store:
@@ -1211,17 +1219,14 @@ Proof.
   inv DEC; try contradiction.
   destruct CASES as [(A & B) | [(A & B) | (A & B)]].
 - (* Same offset *)
-  subst. inv ENC. 
-  assert (chunk = Mint32 \/ chunk = Many32 \/ chunk = Many64)
-  by (destruct chunk; auto || contradiction). 
-  left; split. rewrite H3.
-  destruct H4 as [P|[P|P]]; subst chunk'; destruct v0; simpl in H3; congruence.
+  subst. inv ENC.
+  left; split. rewrite H3. destruct v0; simpl in H3; congruence.
   split. apply compat_pointer_chunks_true; auto.
   auto.
 - (* ofs' > ofs *)
   inv ENC. 
-  + exploit H10; eauto. intros (j & P & Q). inv P. congruence.
-  + exploit H8; eauto. intros (n & P); congruence.
+  + exploit H9; eauto. intros (j & P & Q). inv P. congruence.
+  + exploit H5; eauto. intros (n & P); congruence.
   + exploit H2; eauto. congruence.
 - (* ofs' < ofs *)
   exploit H7; eauto. intros (j & P & Q). subst mv1. inv ENC. congruence.
@@ -1269,6 +1274,7 @@ Proof.
 - contradiction.
 Qed.
 
+(* NOTE: not used
 Lemma store_similar_chunks:
   forall chunk1 chunk2 v1 v2 m b ofs,
   encode_val chunk1 v1 = encode_val chunk2 v2 ->
@@ -1300,6 +1306,7 @@ Theorem store_int16_zero_ext:
   store Mint16 m b ofs (Vint (Int.zero_ext 16 n)) =
   store Mint16 m b ofs (Vint n).
 Proof. intros. apply store_similar_chunks. apply encode_val_int16_zero_ext. auto. Qed.
+*)
 
 (*
 Theorem store_float64al32:
@@ -1563,6 +1570,7 @@ Proof.
   exists m1; split; auto. 
 Qed.
 
+(* NOTE: not used
 Theorem store_int64_split:
   forall m b ofs v m',
   store Mint64 m b ofs v = Some m' ->
@@ -1600,6 +1608,7 @@ Proof.
     omega. apply Int.unsigned_range. auto. exists (two_p (32-3)); reflexivity. 
   change (Int.unsigned (Int.repr 4)) with 4. unfold Int.max_unsigned. omega. 
 Qed.
+*)
 
 (** ** Properties related to [alloc]. *)
 
@@ -1764,7 +1773,9 @@ Theorem load_alloc_same:
 Proof.
   intros. exploit load_result; eauto. intro. rewrite H0. 
   injection ALLOC; intros. rewrite <- H2; simpl. rewrite <- H1.
-  rewrite PMap.gss. destruct chunk; simpl; repeat rewrite ZMap.gi; reflexivity.
+  rewrite PMap.gss. destruct chunk; simpl; repeat rewrite ZMap.gi; try reflexivity.
+  destruct (size_chunk_nat_pos (Mint n)) as [sz EQ]. rewrite EQ.
+  simpl. rewrite ZMap.gi. unfold decode_val. simpl. destruct (eq_nat_dec _ _);subst;auto.
 Qed.
 
 Theorem load_alloc_same':
@@ -3062,8 +3073,8 @@ Record inject' (f: meminj) (m1 m2: mem) : Prop :=
     mi_representable:
       forall b b' delta ofs,
       f b = Some(b', delta) ->
-      perm m1 b (Int.unsigned ofs) Max Nonempty \/ perm m1 b (Int.unsigned ofs - 1) Max Nonempty ->
-      delta >= 0 /\ 0 <= Int.unsigned ofs + delta <= Int.max_unsigned
+      perm m1 b (Int.unsigned 31 ofs) Max Nonempty \/ perm m1 b (Int.unsigned 31 ofs - 1) Max Nonempty ->
+      delta >= 0 /\ 0 <= Int.unsigned 31 ofs + delta <= Int.max_unsigned 31
   }.
 Definition inject := inject'.
 
@@ -3151,24 +3162,24 @@ Qed.
 Lemma address_inject:
   forall f m1 m2 b1 ofs1 b2 delta p,
   inject f m1 m2 ->
-  perm m1 b1 (Int.unsigned ofs1) Cur p ->
+  perm m1 b1 (Int.unsigned 31 ofs1) Cur p ->
   f b1 = Some (b2, delta) ->
-  Int.unsigned (Int.add ofs1 (Int.repr delta)) = Int.unsigned ofs1 + delta.
+  Int.unsigned 31 (Int.add 31 ofs1 (Int.repr 31 delta)) = Int.unsigned 31 ofs1 + delta.
 Proof.
   intros.
-  assert (perm m1 b1 (Int.unsigned ofs1) Max Nonempty) by eauto with mem.
+  assert (perm m1 b1 (Int.unsigned 31 ofs1) Max Nonempty) by eauto with mem.
   exploit mi_representable; eauto. intros [A B].
-  assert (0 <= delta <= Int.max_unsigned).
-    generalize (Int.unsigned_range ofs1). omega.
+  assert (0 <= delta <= Int.max_unsigned 31).
+    generalize (Int.unsigned_range 31 ofs1). omega.
   unfold Int.add. repeat rewrite Int.unsigned_repr; omega.
 Qed.
 
 Lemma address_inject':
   forall f m1 m2 chunk b1 ofs1 b2 delta,
   inject f m1 m2 ->
-  valid_access m1 chunk b1 (Int.unsigned ofs1) Nonempty ->
+  valid_access m1 chunk b1 (Int.unsigned 31 ofs1) Nonempty ->
   f b1 = Some (b2, delta) ->
-  Int.unsigned (Int.add ofs1 (Int.repr delta)) = Int.unsigned ofs1 + delta.
+  Int.unsigned 31 (Int.add 31 ofs1 (Int.repr 31 delta)) = Int.unsigned 31 ofs1 + delta.
 Proof.
   intros. destruct H0. eapply address_inject; eauto. 
   apply H0. generalize (size_chunk_pos chunk). omega. 
@@ -3177,24 +3188,24 @@ Qed.
 Theorem weak_valid_pointer_inject_no_overflow:
   forall f m1 m2 b ofs b' delta,
   inject f m1 m2 ->
-  weak_valid_pointer m1 b (Int.unsigned ofs) = true ->
+  weak_valid_pointer m1 b (Int.unsigned 31 ofs) = true ->
   f b = Some(b', delta) ->
-  0 <= Int.unsigned ofs + Int.unsigned (Int.repr delta) <= Int.max_unsigned.
+  0 <= Int.unsigned 31 ofs + Int.unsigned 31 (Int.repr 31 delta) <= Int.max_unsigned 31.
 Proof.
   intros. rewrite weak_valid_pointer_spec in H0. 
   rewrite ! valid_pointer_nonempty_perm in H0.
   exploit mi_representable; eauto. destruct H0; eauto with mem.
   intros [A B].
-  pose proof (Int.unsigned_range ofs).
+  pose proof (Int.unsigned_range 31 ofs).
   rewrite Int.unsigned_repr; omega.
 Qed.
 
 Theorem valid_pointer_inject_no_overflow:
   forall f m1 m2 b ofs b' delta,
   inject f m1 m2 ->
-  valid_pointer m1 b (Int.unsigned ofs) = true ->
+  valid_pointer m1 b (Int.unsigned 31 ofs) = true ->
   f b = Some(b', delta) ->
-  0 <= Int.unsigned ofs + Int.unsigned (Int.repr delta) <= Int.max_unsigned.
+  0 <= Int.unsigned 31 ofs + Int.unsigned 31 (Int.repr 31 delta) <= Int.max_unsigned 31.
 Proof.
   eauto using weak_valid_pointer_inject_no_overflow, valid_pointer_implies.
 Qed.
@@ -3202,9 +3213,9 @@ Qed.
 Theorem valid_pointer_inject_val:
   forall f m1 m2 b ofs b' ofs',
   inject f m1 m2 ->
-  valid_pointer m1 b (Int.unsigned ofs) = true ->
+  valid_pointer m1 b (Int.unsigned 31 ofs) = true ->
   val_inject f (Vptr b ofs) (Vptr b' ofs') ->
-  valid_pointer m2 b' (Int.unsigned ofs') = true.
+  valid_pointer m2 b' (Int.unsigned 31 ofs') = true.
 Proof.
   intros. inv H1.
   erewrite address_inject'; eauto. 
@@ -3215,9 +3226,9 @@ Qed.
 Theorem weak_valid_pointer_inject_val:
   forall f m1 m2 b ofs b' ofs',
   inject f m1 m2 ->
-  weak_valid_pointer m1 b (Int.unsigned ofs) = true ->
+  weak_valid_pointer m1 b (Int.unsigned 31 ofs) = true ->
   val_inject f (Vptr b ofs) (Vptr b' ofs') ->
-  weak_valid_pointer m2 b' (Int.unsigned ofs') = true.
+  weak_valid_pointer m2 b' (Int.unsigned 31 ofs') = true.
 Proof.
   intros. inv H1.
   exploit weak_valid_pointer_inject; eauto. intros W.
@@ -3225,7 +3236,7 @@ Proof.
   rewrite ! valid_pointer_nonempty_perm in H0.
   exploit mi_representable; eauto. destruct H0; eauto with mem. 
   intros [A B].
-  pose proof (Int.unsigned_range ofs).
+  pose proof (Int.unsigned_range 31 ofs).
   unfold Int.add. repeat rewrite Int.unsigned_repr; auto; omega.
 Qed.
 
@@ -3246,13 +3257,13 @@ Theorem different_pointers_inject:
   forall f m m' b1 ofs1 b2 ofs2 b1' delta1 b2' delta2,
   inject f m m' ->
   b1 <> b2 ->
-  valid_pointer m b1 (Int.unsigned ofs1) = true ->
-  valid_pointer m b2 (Int.unsigned ofs2) = true ->
+  valid_pointer m b1 (Int.unsigned 31 ofs1) = true ->
+  valid_pointer m b2 (Int.unsigned 31 ofs2) = true ->
   f b1 = Some (b1', delta1) ->
   f b2 = Some (b2', delta2) ->
   b1' <> b2' \/
-  Int.unsigned (Int.add ofs1 (Int.repr delta1)) <>
-  Int.unsigned (Int.add ofs2 (Int.repr delta2)).
+  Int.unsigned 31 (Int.add 31 ofs1 (Int.repr 31 delta1)) <>
+  Int.unsigned 31 (Int.add 31 ofs2 (Int.repr 31 delta2)).
 Proof.
   intros. 
   rewrite valid_pointer_valid_access in H1. 
@@ -3261,8 +3272,8 @@ Proof.
   rewrite (address_inject' _ _ _ _ _ _ _ _ H H2 H4). 
   inv H1. simpl in H5. inv H2. simpl in H1.
   eapply mi_no_overlap; eauto.
-  apply perm_cur_max. apply (H5 (Int.unsigned ofs1)). omega.
-  apply perm_cur_max. apply (H1 (Int.unsigned ofs2)). omega.
+  apply perm_cur_max. apply (H5 (Int.unsigned 31 ofs1)). unfold bytesize_chunk, ZRdiv, Zdiv; simpl. omega.
+  apply perm_cur_max. apply (H1 (Int.unsigned 31 ofs2)). unfold bytesize_chunk, ZRdiv, Zdiv; simpl. omega.
 Qed.
 
 Require Intv.
@@ -3311,10 +3322,10 @@ Proof.
   assert (Q: Zabs al <= Zabs sz). apply Zdivide_bounds; auto. omega.
   rewrite Zabs_eq in Q; try omega. rewrite Zabs_eq in Q; try omega.
   assert (R: exists chunk, al = align_chunk chunk /\ al = size_chunk chunk).
-    destruct H0. subst; exists Mint8; auto.
-    destruct H0. subst; exists Mint16; auto.
-    destruct H0. subst; exists Mint32; auto.
-    subst; exists Mint64; auto.
+    destruct H0. subst; exists (Mint 7); auto.
+    destruct H0. subst; exists (Mint 15); auto.
+    destruct H0. subst; exists (Mint 31); auto.
+    subst; exists (Mint 63); auto.
   destruct R as [chunk [A B]].
   assert (valid_access m chunk b ofs Nonempty).
     split. red; intros; apply H3. omega. congruence.
@@ -3344,8 +3355,8 @@ Proof.
   intros. inv H1; simpl in H0; try discriminate.
   exploit load_inject; eauto. intros [v2 [LOAD INJ]].
   exists v2; split; auto. unfold loadv. 
-  replace (Int.unsigned (Int.add ofs1 (Int.repr delta)))
-     with (Int.unsigned ofs1 + delta).
+  replace (Int.unsigned 31 (Int.add 31 ofs1 (Int.repr 31 delta)))
+     with (Int.unsigned 31 ofs1 + delta).
   auto. symmetry. eapply address_inject'; eauto with mem.
 Qed.
 
@@ -3444,8 +3455,8 @@ Theorem storev_mapped_inject:
 Proof.
   intros. inv H1; simpl in H0; try discriminate.
   unfold storev.
-  replace (Int.unsigned (Int.add ofs1 (Int.repr delta)))
-    with (Int.unsigned ofs1 + delta).
+  replace (Int.unsigned 31 (Int.add 31 ofs1 (Int.repr 31 delta)))
+    with (Int.unsigned 31 ofs1 + delta).
   eapply store_mapped_inject; eauto.
   symmetry. eapply address_inject'; eauto with mem.
 Qed.
@@ -3618,8 +3629,8 @@ Theorem alloc_left_mapped_inject:
   inject f m1 m2 ->
   alloc m1 lo hi = (m1', b1) ->
   valid_block m2 b2 ->
-  0 <= delta <= Int.max_unsigned ->
-  (forall ofs k p, perm m2 b2 ofs k p -> delta = 0 \/ 0 <= ofs < Int.max_unsigned) ->
+  0 <= delta <= Int.max_unsigned 31 ->
+  (forall ofs k p, perm m2 b2 ofs k p -> delta = 0 \/ 0 <= ofs < Int.max_unsigned 31) ->
   (forall ofs k p, lo <= ofs < hi -> perm m2 b2 (ofs + delta) k p) ->
   inj_offset_aligned delta (hi-lo) ->
   (forall b delta' ofs k p,
@@ -3681,10 +3692,10 @@ Proof.
    subst. injection H9; intros; subst b' delta0. destruct H10.
     exploit perm_alloc_inv; eauto; rewrite dec_eq_true; intro.
     exploit H3. apply H4 with (k := Max) (p := Nonempty); eauto.
-    generalize (Int.unsigned_range_2 ofs). omega.
+    generalize (Int.unsigned_range_2 31 ofs). omega.
    exploit perm_alloc_inv; eauto; rewrite dec_eq_true; intro.
    exploit H3. apply H4 with (k := Max) (p := Nonempty); eauto.
-   generalize (Int.unsigned_range_2 ofs). omega.
+   generalize (Int.unsigned_range_2 31 ofs). omega.
   eapply mi_representable0; try eassumption.
   destruct H10; eauto using perm_alloc_4.
 (* incr *)
@@ -3713,7 +3724,7 @@ Proof.
   eapply alloc_right_inject; eauto.
   eauto.
   instantiate (1 := b2). eauto with mem.
-  instantiate (1 := 0). unfold Int.max_unsigned. generalize Int.modulus_pos; omega.
+  instantiate (1 := 0). unfold Int.max_unsigned. generalize (Int.modulus_pos 31); omega.
   auto.
   intros. apply perm_implies with Freeable; auto with mem.
   eapply perm_alloc_2; eauto. omega.
@@ -3917,13 +3928,13 @@ Proof.
   destruct (f b) as [[b1 delta1] |] eqn:?; try discriminate.
   destruct (f' b1) as [[b2 delta2] |] eqn:?; inv H. 
   exploit mi_representable0; eauto. intros [A B].
-  set (ofs' := Int.repr (Int.unsigned ofs + delta1)).
-  assert (Int.unsigned ofs' = Int.unsigned ofs + delta1). 
+  set (ofs' := Int.repr 31 (Int.unsigned 31 ofs + delta1)).
+  assert (Int.unsigned 31 ofs' = Int.unsigned 31 ofs + delta1). 
     unfold ofs'; apply Int.unsigned_repr. auto.
   exploit mi_representable1. eauto. instantiate (1 := ofs').
   rewrite H.
-  replace (Int.unsigned ofs + delta1 - 1) with
-    ((Int.unsigned ofs - 1) + delta1) by omega.
+  replace (Int.unsigned 31 ofs + delta1 - 1) with
+    ((Int.unsigned 31 ofs - 1) + delta1) by omega.
   destruct H0; eauto using perm_inj.
   rewrite H. omega.
 Qed.
@@ -4027,7 +4038,7 @@ Proof.
   apply flat_inj_no_overlap.
 (* range *)
   unfold flat_inj; intros.
-  destruct (plt b (nextblock m)); inv H0. generalize (Int.unsigned_range_2 ofs); omega.
+  destruct (plt b (nextblock m)); inv H0. generalize (Int.unsigned_range_2 31 ofs); omega.
 Qed.
 
 Theorem empty_inject_neutral:
